day1/checker.fsti
@@ -3,8 +3,9 @@ module Checker
 open Try
 open Ast
 
-val size        : (#a:Type) -> term a -> nat
+val size       : #a:Type -> term a -> nat
+val closed     : #a:Type -> nat -> e:term a -> Tot bool (decreases %[size e])
 
-val typeInfer   : nat -> context -> (e:term infer) -> Tot (result typeL) (decreases (size e))
-val typeCheck   : nat -> context -> (e:term check) -> (t:typeL) -> Tot (result unit) (decreases %[size e;t])
-val typeInfer0  : context -> term infer -> result typeL
+val typeInfer  : n:nat -> context -> e:(term infer){closed n e} -> Tot (result typeL) (decreases (size e))
+val typeCheck  : n:nat -> context -> e:(term check){closed n e} -> t:typeL -> Tot (result unit) (decreases %[size e;t])
+val typeInfer0 : context -> e:(term infer){closed 0 e} -> result typeL
