day1/closed.fsti
@@ -1,7 +1,0 @@
-module Closed
-
-open Try
-open Ast
-
-val closed : (#a:Type) -> list nat -> e:term a -> Tot bool // (decreases e)
-
