day1/size.fsti
@@ -1,5 +1,0 @@
-module Size
-
-open Ast
-
-val size : (#a:Type) -> term a -> nat
